Refactor LabelsDefined to own module.

CopyPropagation.v
@@ -1,7 +1,7 @@
 Require Import CSet Le.
 
 Require Import Plus Util AllInRel Map.
-Require Import Val Var Env EnvTy IL Sim Alpha Coherence Fresh Annotation DecSolve SetOperations.
+Require Import Val Var Env EnvTy IL Sim Alpha Coherence Fresh Annotation DecSolve SetOperations LabelsDefined.
 
 Require Import Liveness ValueOpts.
 
@@ -183,43 +183,6 @@ Qed.
 Print Instances Proper.
 
 
-Inductive labelsDefined (A:Type) : stmt -> list A -> Prop :=
-  | labelsDefinedExp x e s L
-    : labelsDefined s L
-      -> labelsDefined (stmtExp x e s) L
-  | labelsDefinedIf e s t L
-    : labelsDefined s L
-      -> labelsDefined t L
-      -> labelsDefined (stmtIf e s t) L
-  | labelsDefinedRet e L
-    : labelsDefined (stmtReturn e) L
-  | labelsDefinedGoto f Y a L
-    : get L (counted f) a
-      -> labelsDefined (stmtGoto f Y) L
-  | labelsDefinedExtern x f Y s L
-    : labelsDefined s L
-      -> labelsDefined (stmtExtern x f Y s) L
-  | labelsDefinedLet s t Z L a
-    :  labelsDefined s (a::L)
-      -> labelsDefined t (a::L)
-      -> labelsDefined (stmtLet Z s t) L.
-
-Lemma labelsDefined_any A (L:list A) (L':list A) s
-: length L = length L'
-  -> labelsDefined s L
-  -> labelsDefined s L'.
-Proof.
-  intros. eapply length_length_eq in H.
-  general induction H0; eauto using labelsDefined.
-  - edestruct get_length_eq.
-    eauto. eapply length_eq_length; eauto.
-    econstructor; eauto.
-  - econstructor.
-    eapply IHlabelsDefined1; eauto.
-    instantiate (1:=a). econstructor; eauto.
-    eapply IHlabelsDefined2; eauto.
-    econstructor; eauto.
-Qed.
 
 
 Lemma single_in_cp_eqns x ϱ D
