IL/LabelsDefined.v
@@ -1,0 +1,49 @@
+Require Import List.
+Require Import Util Relations Get Drop Var Val Exp Env Map CSet AutoIndTac MoreList IL DecSolve.
+
+Set Implicit Arguments.
+
+Inductive labelsDefined (A:Type) : stmt -> list A -> Prop :=
+  | labelsDefinedExp x e s L
+    : labelsDefined s L
+      -> labelsDefined (stmtExp x e s) L
+  | labelsDefinedIf e s t L
+    : labelsDefined s L
+      -> labelsDefined t L
+      -> labelsDefined (stmtIf e s t) L
+  | labelsDefinedRet e L
+    : labelsDefined (stmtReturn e) L
+  | labelsDefinedGoto f Y a L
+    : get L (counted f) a
+      -> labelsDefined (stmtGoto f Y) L
+  | labelsDefinedExtern x f Y s L
+    : labelsDefined s L
+      -> labelsDefined (stmtExtern x f Y s) L
+  | labelsDefinedLet s t Z L a
+    :  labelsDefined s (a::L)
+      -> labelsDefined t (a::L)
+      -> labelsDefined (stmtLet Z s t) L.
+
+Lemma labelsDefined_any A (L:list A) (L':list A) s
+: length L = length L'
+  -> labelsDefined s L
+  -> labelsDefined s L'.
+Proof.
+  intros. eapply length_length_eq in H.
+  general induction H0; eauto using labelsDefined.
+  - edestruct get_length_eq.
+    eauto. eapply length_eq_length; eauto.
+    econstructor; eauto.
+  - econstructor.
+    eapply IHlabelsDefined1; eauto.
+    instantiate (1:=a). econstructor; eauto.
+    eapply IHlabelsDefined2; eauto.
+    econstructor; eauto.
+Qed.
+
+
+(*
+*** Local Variables: ***
+*** coq-load-path: (("../" "Lvc")) ***
+*** End: ***
+*)
